\subsection*{Problem 2.7}
Assume that $V$ is a vector space.  By the vector space axioms, for each $v\in V$, there exists an additive inverse, which we denote $(-v)$. This additive inverse $(-v)$ is unique (see LADR 1.26). Since $(-v)$ is in $V$, it too has an additive inverse, which we will write as $-(-v)$.  Prove that
	\begin{align*}
		-(-v)=v.
	\end{align*}
\renewcommand\qedsymbol{$\blacksquare$}
\begin{proof}
    Let $v\in V$ and $w$ be the additive inverse of $-v$. Then,
    \[
        w+(-v)=\vec{0},
    \]
    or $v+w+(-v)=v$. From the commutative and associative property of vector addition,
    \[
        \begin{aligned}
        v &= v+w+(-v)\\
          &= w+v+(-v)\\
          &= w+(v+(-v))\\
          &= w+\vec{0}\\
          &= w
        \end{aligned}
    \]
    (since $-v$ is the additive inverse of $v$). Therefore, $-(-v)=w=v$
\end{proof}