\begin{question}
	\normalfont

Consider the polynomials	\begin{align*}
		p_1(x) = 1-x,\ \ \ \ p_2(x)=x^2+x,\ \ \ \ p_3(x)=x^3+x^2,\ \ \ \ p_4(x)=x^3.
	\end{align*}
	For the polynomial, $g\in\P_3$, given by
	\begin{align*}
		g(x)=2x^3+1,
	\end{align*}
	produce a list of real numbers, $\al_1$, $\al_2$, $\al_3$, $\al_4$, so that
	\begin{align*}
		g = \al_1 p_1 + \al_2 p_2 + \al_3 p_3 + \al_4 p_4.
	\end{align*}

\end{question}

\begin{sol}
    Let $\al_1,\al_2,\al_3,\al_4\in\R$ be a solution to $g=\al_1p_1+\al_2p2+\al_3p_3+\al_4p_4$. It follows that 
    \[
        \begin{aligned}
            g &= \al_1p_1+\al_2p_2+\al_3p_3+\al_4p_4\\
              &= \al_1(1-x)+\al_2(x^2+x)+\al_3(x^3+x^2)+\al_4(x^3)\\
              &= \al_1-\al_1x+\al_2x^2+\al_2x+\al_3x^3+\al_3x^2+\al_4x^3\\
              &= \al_1+(\al_2-\al_1)x+(\al_2+\al_3)x^2+(\al_3+\al_4)x^3\\
              &= 2x^3+1
        \end{aligned}
    \]
    We can convert the equation to the following system of equations:
    \begin{align*}
        \begin{cases}
            \al_1       &= 1\\
            \al_2-\al_1 &= 0\\
            \al_2+\al_3 &= 0\\
            \al_3+\al_4 &= 2
        \end{cases}
        \iff
        \begin{cases}
            \al_1 &= 1\\
            \al_2 &= \al_1\\
            \al_3 &= -\al_2\\
            \al_4 &= 2-\al_3
        \end{cases}\\
        \iff
        (\al_1,\al_2,\al_3,\al_4)=(1,1,-1,3)
    \end{align*}
    Therefore, $(\al_1,\al_2,\al_3,\al_4)=(1,1,-1,3)$ satisfies the problem statement.
\end{sol}
