\begin{question}
    \normalfont
    Prove, using induction, that for all $n\in\N$ the following equality holds.
    \[
        \begin{aligned}
            \sum_{i=1}^{n}\frac{2}{(i+1)(i+2)}=\frac{n}{n+2}
        \end{aligned}
    \]
\end{question}

\begin{proof}
    \renewcommand{\qedsymbol}{$\blacksquare$}
    Let $P(n)$ be defined as 
    \[
        \begin{aligned}
            \forall n\in\N, P(n)\iff \sum_{i=1}^{n}\frac{2}{(i+1)(i+2)}=\frac{n}{n+2}
        \end{aligned}
    \]
    We will show that $P(n)$ holds for all $n\in\N$.

    Base case: When n=1, 
    \[
        \begin{aligned}
            \sum_{i=1}^{n}\frac{2}{(i+1)(i+2)}=\frac{2}{6}=\frac{1}{1+3}
        \end{aligned}
    \]
    , or $P(n)$ holds for the base case.

    Induction step: Assume $P(n)$ holds for some $n=k\in\N$. We will show that $P(n+1)$ holds.
    Since $P(k)$ holds, 
    \[
        \begin{aligned}
            \sum_{i=1}^{k}\frac{2}{(i+1)(i+2)}=\frac{k}{k+2}
        \end{aligned}
    \]
    We have 
    \[
        \begin{aligned}
            &\quad\, \sum_{i=1}^{k+1}\frac{2}{(i+1)(i+2)}\\
            &= \sum_{i=1}^{k}\frac{2}{(i+1)(i+2)}+\frac{2}{(k+1+1)(k+1+2)}\\
            &= \frac{k}{k+2}+\frac{2}{(k+2)(k+3)}\\
            &= \frac{k(k+3)}{(k+2)(k+3)}+\frac{2}{(k+2)(k+3)}\\
            &= \frac{k^2+3k+2}{(k+2)(k+3)}\\
            &= \frac{(k+1)(k+2)}{(k+2)(k+3)}\\
            &= \frac{k+1}{k+3}\\
            &= \frac{k+1}{(k+1)+2}
        \end{aligned}
    \]
    Hence, $\mathlarger{\sum_{i=1}^{k+1}\frac{2}{(i+1)(i+2)}=\frac{k+1}{(k+1)+2}}$, or $P(n)$ holds for $n=k+1$. Therefore, from the principle of mathematical induction, it follows that for every $n\in\N$, 
    \[
        \begin{aligned}
            \sum_{i=1}^{n}\frac{2}{(i+1)(i+2)}=\frac{n}{n+2}
        \end{aligned}
    \]
\end{proof}