\begin{question}
	\normalfont
	
	Suppose $T \in \mathcal{L}(U,V)$ and $S \in \mathcal{L}(V,W)$ are both invertible linear maps. Prove that $ST \in \mathcal{L}(U,W)$ is invertible and that $(ST)^{-1} = T^{-1}S^{-1}$. 
	
	
	\end{question}
\begin{proof}
    \renewcommand{\qedsymbol}{$\blacksquare$}
    Let $T\in\mathcal{L}(U,V)$ and $S\in\mathcal{L}(V,W)$ be invertible and $id_U,id_V,id_W$ be the identity linear transformation for $U,V,W$, respectively.
    Then, there exist $T^{-1}\in\mathcal{L}(V,U)$ and $S^{-1}\in\mathcal{L}(W,V)$ such that $TT^{-1}=S^{-1}S=id_V, \ T^{-1}T=id_U \text{ and } SS^{-1}=id_W$.

    Moreover, since $S^{-1}\in\mathcal{L}(W,V)$ and $id_V\in\mathcal{L}(V,V)$, $id_V S^{-1}$ is defined and $id_V S^{-1}=S^{-1}$.
    Similarly, $id_V T$ is defined and $id_V T=T$.\\
    From the definition of $T$ and $S$, it follows that $ST\in\mathcal{L}(U,W)$. Hence,
    \[
        \begin{aligned}
            (ST)(T^{-1}S^{-1})
            = S((TT^{-1})S^{-1})
            = S(id_VS^{-1})
            = SS^{-1}=id_W
        \end{aligned}
    \]
    and 
    \[
        \begin{aligned}
            (T^{-1}S^{-1})(ST)
            = T^{-1}((S^{-1}S)T)
            = T^{-1}(id_VT)
            = T^{-1}T=id_U
        \end{aligned}
    \]
    Thus, $T^{-1}S^{-1}$ is both the left inverse and right inverse of $ST$, or $ST$ is invertible and $(ST)^{-1}=T^{-1}S^{-1}$.
\end{proof}