\begin{question}
	\normalfont
	
	Use mathematical induction to prove the following statement:
	\begin{align*}
		\textnormal{for all}\ n\in\Natural,\ \ 
		\MatTwoTwo{2}{0}{-1}{1}^n
		= \MatTwoTwo{2^n}{0}{1-2^n}{1}.
	\end{align*}
\end{question}

\begin{proof}
    \renewcommand{\qedsymbol}{$\blacksquare$}
    Let $P(n)$ be defined as the statement 
    \[
        \begin{aligned}
            \MatTwoTwo{2}{0}{-1}{1}^n=\MatTwoTwo{2^n}{0}{1-2^n}{1}
        \end{aligned}
    \]
    for all $n\in\N$. 

    Base case: Consider $n=1\in\N$. Then 
    \[
        \begin{aligned}
            \MatTwoTwo{2}{0}{-1}{1}^n=\MatTwoTwo{2}{0}{-1}{1}=\MatTwoTwo{2^n}{0}{1-2^n}{1}
        \end{aligned}
    \]
    , or $P(1)$ is true.

    Induction step: Assume $P(n)$ is true for some $n=k\in\N$. That is, $P(k)$ is true, or 
    \[
        \begin{aligned}
            \MatTwoTwo{2}{0}{-1}{1}^k=\MatTwoTwo{2^k}{0}{1-2^k}{1}
        \end{aligned}
    \] 
    We have: the statement $P(k+1)$ is 
    \[
        \begin{aligned}
            \MatTwoTwo{2}{0}{-1}{1}^{k+1}=\MatTwoTwo{2^{k+1}}{0}{1-2^{k+1}}{1}
        \end{aligned}
    \]
    However,
    \[
        \begin{aligned}
            &\MatTwoTwo{2}{0}{-1}{1}^{k+1}\\
            =&\MatTwoTwo{2}{0}{-1}{1}^k\MatTwoTwo{2}{0}{-1}{1}\\
            =&\MatTwoTwo{2^k}{0}{1-2^k}{1}\MatTwoTwo{2}{0}{-1}{1}\\
            =&\MatTwoTwo{2^{k+1}+0\times-1}{2^k\times 0+0\times 1}{2-2^{k+1}-1}{0(1-2^k)+1\times 1}\\
            =&\MatTwoTwo{2^{k+1}}{0}{1-2^{k+1}}{1}
        \end{aligned}
    \]
    Hence, $P(k+1)$ must also be true.

    From the principle of mathematical induction, it follows that the statement $P(n)$ is true for all $n\in\N$.
\end{proof}