\begin{question}
\normalfont
Let $S$ be an invertible $l \times l$ matrix and $D$ be an $l \times l$ matrix. Use mathematical induction to prove 
$$
\left(S D S^{-1} \right)^n = S D^n S^{-1}, \text{ for all } n \in \mathbb{N}.
$$ 
\end{question}

\begin{proof}
    \renewcommand{\qedsymbol}{$\blacksquare$}
    For all $n\in\N$, let $P(n)$ be defined as
    \[
        \begin{aligned}
            P(n)\iff(SDS^{-1})^n=SD^nS^{-1}
        \end{aligned}
    \] 
    
    Base case: When $n=1$, $(SDS^{-1})^1=SD^1S^{-1}$, or $P(1)$ holds.

    Induction step: Let $k\in\N$ and assume $P(n)$ holds for $n=k$.
    Let $I_k$ be the $k\times k$ identity matrix.
    Then, $(SDS^{-1})^k=SD^kS^{-1}$ and for $n=k+1$, 
    \[
        \begin{aligned}
            &(SDS^{-1})^{k+1}
            =(SDS^{-1})^k(SDS^{-1})
            =(SD^kS^{-1})(SDS^{-1})
            =(SD^k)(S^{-1}S)(DS^{-1})\\
            =&(SD^k)(I_kDS^{-1})
            =SD^kDS^{-1}
            =SD^{k+1}S^{-1}
        \end{aligned}
    \]
    Hence, $P(k+1)$ holds. From the principle of mathematical induction, it follows that $P(n)$ holds for all $n\in\N$.\qed
    \renewcommand{\qedsymbol}{}
\end{proof}